update tutorial, some bugfixes in Autosubst.v

examples/demo.v
@@ -1,102 +1,198 @@
-Require Import Autosubst Contexts.
+(** * Tutorial
 
-(** 
-The inductive definition of term contains annotations for the automatic generation of the substitution.
+    In this tutorial we will use Autosubst to formalize substitutivity and
+    subject reduction in the simply typed lambda calculus. *)
 
-"var" is convertible to nat and indicates the constructor used for variables.
-There should be exactly one such constructor and it should only have a single argument, which must be of type var.
+Require Import Autosubst List.
 
-"bind T" is convertible to T and indicates that a variable is bound in the respective subterm.
-*)
+(** ** Syntax and the substitution operation
+
+    Types and terms of the simply typed lambda calculus are described by the
+    following grammar.
+
+<<
+  A, B ::= * | A -> B
+  s, t ::= x | s t | \ A. s
+>>
+
+    Types are either the base type, or a function type. Terms are variables,
+    applications, or abstractions. In order to generate the substitution
+    operation for terms we will add some annotations to terms. In this case we
+    will have to mark the variable and abstraction constructor with the
+    following constructs:
+
+    - [var] is convertible to [nat] and indicates the constructor used for
+      variables.
+    - [{bind T}] is convertible to [T] and indicates that a variable is bound in
+      the respective subterm. *)
+
+Inductive type :=
+| TBase
+| TFun  (A B : type).
 
 Inductive term :=
 | TVar (x : var)
-| Lam (s : {bind term})
-| App (s t : term)
-.
+| App  (s t : term)
+| Lam  (A : type) (s : {bind term}).
 
-(* Now we can fully automatically derive the substitution operations and the corresponding lemmas. This is done by generating instances for the typeclasses Subst and SubstLemmas.
+(** Now we can automatically derive the substitution operations and lemmas.
+    This is done by generating instances for the following typeclasses:
+    - [VarConstr term] provides the generic variable constructor Var for term.
+      It is always equivalent to the single constructor having an argument of
+      type [var]. In this example, [Var] is convertible to [TVar].
+    - [Rename term] provides the renaming operation on term.
+    - [Subst term] provides the substitution operation on term and needs a
+      [Rename] instance in the presence of binders.
+    - [SubstLemmas term] contains proofs for the basic lemmas.
 
-(Subst term) contains the following operations:
-  - subst : (var -> term) -> term -> term
-    the generic substitution operation
-  - Var : var -> term
-    a generic term constructor for variables. It is always identical to the single constructor having an argument of type "var". So in this example, "Var" is convertible to "TVar".
-  - rename : (var -> var) -> term -> term
-    a renaming operations. It is only needed for technical reasons and subsumed by subst. It is mostly hidden in the interface and you should not stumble upon it.
+    Each instance is inferred automatically by using the [derive] tactic. *)
 
-We define the notations:
-  - "s.[sigma]" for (subst sigma s)
-  - "sigma >> tau" for the composition of sigma and tau, that is, (fun x => (sigma x).[tau])
+Instance VarConstr_term : VarConstr term. derive. Defined.
+Instance Rename_term : Rename term. derive. Defined.
+Instance Subst_term : Subst term. derive. Defined.
+Instance SubstLemmas_term : SubstLemmas term. derive. Qed.
 
-SubstLemmas contains the following lemmas:
-  - subst_comp : forall (s : term) (sigma tau : var -> term), s.[sigma].[tau] = s.[sigma >> tau]
-  - subst_id : forall s : term, s.[Var] = s
-  - id_subst : forall (x : var) (sigma : var -> term), (Var x).[sigma] = sigma x
-  - rename_subst : forall (xi : var -> var) (s : term), rename xi s = s.[ren xi]
-where
-  ren xi x = Var (xi x)
-*)
+(** At this point we can use the notations:
+    - [s.[sigma]] for the application of the substitution sigma to a term s.
+    - [sigma >> tau] for the composition of sigma and tau, i.e., the
+      substitution [fun x => (sigma x).[tau]].
 
-Instance VarConstr_term : VarConstr term. derive_VarConstr. Defined.
-Instance Rename_term : Rename term. derive_Rename. Defined.
-Instance Subst_term : Subst term. derive_Subst. Defined.
-Instance substLemmas_term : SubstLemmas term. derive_SubstLemmas. Qed.
+    SubstLemmas contains the following lemmas:
+    - id_subst s x : [(Var x).[sigma] = sigma x]
+    - subst_id s : [s.[Var] = s]
+    - subst_comp sigma tau : [s.[sigma].[tau] = s.[sigma >> tau]]
+    - rename_subst xi s : [rename xi s = s.[ren xi]]
+    where [ren xi x = Var (xi x)].
 
+    In addition these lemmas allow you to use the autosubst tactic. *)
+
+(** ** Reduction and substitutivity
+
+    Reductions are defined by the following inference rules:
+
+<<
+    s1 \rhd s2        t1 \rhd t2          s1 \rhd s2
+  --------------    --------------    ------------------
+  s1 t \rhd s2 t    s t1 \rhd s t2    \A. s1 \rhd \A. s2
+
+
+  ---------------------------
+  (\A. s) t \rhd s.[beta t]
+>>
+
+    Where [beta t] is notation for the substitution [t .: Var].
+
+    The definition below is an almost verbatim copy of the inference rules. The
+    one difference is in the beta rule. Instead of using [s.[beta t]]
+    directly, we add an equation to the premise.
+
+<<
+   s2 = s1.[beta t]
+  ------------------
+  (\A. s1) t \rhd s2
+>>
+
+    This makes the constructor applicable even if the substitution on [s] is not
+    of to the special form [t .: Var]. *)
 
 Inductive step : term -> term -> Prop :=
-| Step_Beta s s' t : s' = s.[t .: Var] -> step (App (Lam s) t) s'
-| Step_App1 s s' t: step s s' -> step (App s t) (App s' t)
-| Step_App2 s t t': step t t' -> step (App s t) (App s t')
-| Step_Lam s s' : step s s' -> step (Lam s) (Lam s')
-.
+| Step_Beta (A : type) (s1 s2 t : term) :
+    s2 = s1.[beta t] -> step (App (Lam A s1) t) s2
+| Step_App1 (s1 s2 t : term) :
+    step s1 s2 -> step (App s1 t) (App s2 t)
+| Step_App2 (s t1 t2 : term) :
+    step t1 t2 -> step (App s t1) (App s t2)
+| Step_Lam (A : type) (s1 s2 : term) :
+    step s1 s2 -> step (Lam A s1) (Lam A s2).
 
-Inductive type :=
-| Base
-| Arr (A B : type)
-.
+Lemma step_subst s1 s2 :
+  step s1 s2 -> forall sigma, step s1.[sigma] s2.[sigma].
+Proof.
+(** The proof of substitutivity proceeds by induction on the step relation.
+    Every case, except for [Step_Beta] is trivial and solved by eauto. *)
+  induction 1; eauto using step.
+(** In the beta case we can apply the constructor and simplify the goal. *)
+  intros sigma. autosubst. constructor. subst.
+(** At this point our goal is to show the equation:
+<<
+   s1.[beta t].[sigma] = s1.[up sigma].[beta t.[sigma]]
+>>
+    This is a parallel variant of Barendregt's famous substitution lemma.
+    As it is simply an equations between terms with substitutions we can solve
+    this goal using autosubst. In this particular case, the equation holds
+    because both sides are equivalent to the normal form
+    [s1.[t.[sigma] .: sigma]]. *)
+  now autosubst.
+Qed.
+
+(** ** Type preservation
+
+    The typing relation is defined by the following inference rules.
+
+<<
+   Gamma x = A      Gamma |- s : A -> B    Gamma |- t : A
+  --------------   ---------------------------------------
+  Gamma |- x : A             Gamma |- s t : B
+
+      Gamma, A |- s : B
+  -------------------------
+   Gamma |- \A. s : A -> B
+>>
+
+    We implement contexts as lists and write [A :: Gamma] instead of "Gamma, A".
+    Apart from this, we also need to implement the "Gamma x = A" line in the
+    variable rule. Since this is just a list lookup we use the [nth_error]
+    function from the list library. *)
 
 Inductive ty (Gamma : list type) : term -> type -> Prop :=
-| Ty_Var x A : atn Gamma x A -> ty Gamma (Var x) A
-| Ty_Lam s A B: ty (A :: Gamma) s B -> ty Gamma (Lam s) (Arr A B)
-| Ty_App s t A B: ty Gamma s (Arr A B) -> ty Gamma t A -> ty Gamma (App s t) B
-.
+| Ty_Var (x : var) (A : type) :
+    nth_error Gamma x = value A -> ty Gamma (Var x) A
+| Ty_App (A B : type) (s t : term) :
+    ty Gamma s (TFun A B) -> ty Gamma t A -> ty Gamma (App s t) B
+| Ty_Lam (A B : type) (s : term) :
+    ty (A :: Gamma) s B -> ty Gamma (Lam A s) (TFun A B).
 
-(** The library defines the tactic autosubst, which simplifies expressions containing substitutions and tries to compute a normal form for substitutions. 
-*)
+(** Our goal for the rest of the tutorial is to show type preservation, that is:
+<<
+  Gamma |- s : A -> s \rhd t -> Gamma |- t : A
+>>
+    As usual, this requires a substitution lemma, which in turn requires
+    weakening. Using parallel substitutions we can show a general lemma for
+    arbitrary substitutions. The weakening lemma is the special case of a
+    renaming substitution. *)
 
-(** This subsumes the usual weakening and reordering lemmas. Context extension and reordering is expressed with the renaming xi, which maps indices referring to the original context to indices referring to the extended context. 
-*)
-
-Lemma ty_weak Gamma1 s A:
-  ty Gamma1 s A -> forall xi Gamma2,
-  (forall x B, atn Gamma1 x B -> atn Gamma2 (xi x) B) ->
-  ty Gamma2 s.[ren xi] A.
+Lemma ty_weak Gamma s A :
+  ty Gamma s A -> forall Delta xi,
+  (forall x B,
+     nth_error Gamma x = value B -> nth_error Delta (xi x) = value B) ->
+  ty Delta s.[ren xi] A.
 Proof.
   induction 1; intros; autosubst; eauto using ty.
   constructor. apply IHty. intros [|]; simpl; eauto.
 Qed.
 
-
-(** This is the usual substitutivity lemma for the typing relation extended to parallel substitutions.
-*)
-Lemma ty_subst Gamma1 s A : 
-  ty Gamma1 s A -> forall sigma Gamma2,
-  (forall x B, atn Gamma1 x B -> ty Gamma2 (sigma x) B) ->
-  ty Gamma2 s.[sigma] A.
+Lemma ty_subst Gamma s A :
+  ty Gamma s A -> forall Delta sigma,
+  (forall x B, nth_error Gamma x = value B -> ty Delta (sigma x) B) ->
+  ty Delta s.[sigma] A.
 Proof.
   induction 1; intros; autosubst; eauto using ty.
   constructor. apply IHty. intros [|]; simpl; eauto using ty, ty_weak.
 Qed.
 
-Lemma preservation s t: step s t -> forall A Gamma, ty Gamma s A -> ty Gamma t A.
+Lemma substitution Gamma s t A B :
+  ty (A :: Gamma) s B ->
+  ty Gamma t A ->
+  ty Gamma s.[beta t] B.
 Proof.
-  induction 1; intros; ainv; eauto using ty.
-  eapply ty_subst; eauto.
-  intros [|]; simpl; intros; subst; eauto using ty.
+  intros T1 T2. apply (ty_subst _ _ _ T1). intros [|x] C; simpl; eauto using ty.
+  intros H. inversion H; subst; auto.
 Qed.
 
-Lemma step_subst s s' : step s s' -> forall sigma, step s.[sigma] s'.[sigma].
+Lemma preservation s t :
+  step s t -> forall Gamma A, ty Gamma s A -> ty Gamma t A.
 Proof.
-  induction 1; autosubst; constructor; subst; trivial. now autosubst.
+  induction 1 as [A' s1 s2 t e|s1 s2 t _ ih|s t1 t2 _ ih|A s1 s2 _ ih];
+    intros Gamma B T; inversion_clear T; eauto using ty; subst.
+  inversion_clear H. revert H1 H0. apply substitution.
 Qed.
